\begin{align*}
    U_{k+1} &= U_k + 2k + 3 \quad ,k \ge 0 \quad ,U_o=1 \\
    U_k &= U_{k-1} + 2(k-1) + 3 \quad ,(k-1) \ge 0\\
    U_k &= U_{k-1} + 2k + 1 \quad ,k \ge 1\\
    U_k - U_{k-1} &=  2k + 1\quad \text{/}\cdot\sumatoria{i=1}{k}\\
    \sumatoria{i=1}{k}(U_i - U_{i-1}) &= \sumatoria{i=1}{k} 2i +\sumatoria{i=1}{k} 1 \\
    U_k - U_0 &= 2\sumatoria{i=1}{k}i + \sumatoria{i=1}{k}1\\
    U_k - 1 &= 2 \left( \frac{k(k+1)}{2} \right) + k \\
    U_k &= k^2 +2k + 1 \\
    \therefore U_k &= (k+1)^2 \quad k \ge 0
\end{align*}